compiler/src/compiler/SeparationLogic.v
@@ -70,7 +70,7 @@ Section ptstos.
   Context {W: Words}.
   Context {mem : map.map word byte} {mem_ok: map.ok mem}.
 
-  Definition bytes_per_word: Z := Z.of_nat (@Memory.bytes_per width Syntax.access_size.word).
+  Definition bytes_per_word: Z := Memory.bytes_per_word width.
 
   Definition word_array: word -> list word -> mem -> Prop :=
     array ptsto_word (word.of_Z bytes_per_word).
